\begin{document}
\extrawidth{0.5in} \extrafootheight{-0in} \pagestyle{headandfoot}
\headrule \header{\textbf{cs2311 - Fall 2014}}{\textbf{HW
 8 \ifprintanswers - Solutions \fi}}{\textbf{Due: Wed 11/12/14}} \footrule \footer{}{Page \thepage\
of \numpages}{}

\ifprintanswers
% \noindent You should \underline{complete all problems}, but \underline{only a subset will be graded} (which will be graded is not known to you ahead of time). 
\else
\noindent \textbf{Instructions:} All assignments are due \underline{by \textbf{4pm} on the due date} specified.  There will be a box in the CS department office (Rekhi 221) where assignments may be turned in.  Solutions will be posted on-line at the following lecture.  Every student
must write up their own solutions in their own manner.

\medskip
\noindent Please present your solutions in a clean, understandable
manner; pages should be stapled before being turned in, no ragged edges of
paper.

% \medskip
% \noindent Be clear with you penmanship to distinguish set brackets and parentheses.
%   For example, $\{1, 2\}$ is a set where $(1,2)$ is an ordered pair.  Also,
% differentiate the empty set $\emptyset$ and the number zero 0.

\medskip
\noindent You should \underline{complete all problems}, but \underline{only a subset will be graded} (which will be graded is not known to you ahead of time). 
\fi

\begin{questions}

\uplevel{{\bf Sequences}}

\gquestion{10}{6}{(a,c,e)} What are the first 4 terms of each sequence:

\begin{tabular}{ll}
    (a) $a_n = 4-2n\;\;\forall n \geq 0$ \hspace{0.35in} 
        & (b) $b_n = 6- 3\cdot 2^n \;\;\forall n \geq 0$ \\
    (c) $c_1 = 4,  c_n = 3\cdot c_{n-1} - 2 \;\; \forall n \geq 2$ \hspace{0.3in}
        & (d) $d_1 = -1, d_n = 5\cdot d_{n-1} + 1\;\; \forall n \geq 2$ \\
    \multicolumn{2}{c}{(e) $e_0 = 1, e_1 = 1$, $e_n = ne_{n-1} + n^2e_{n-2} \;\forall n \geq 2$}
\end{tabular}
    \ifprintanswers
        \vspace{-10pt}
   \fi
\begin{solution}

    \begin{tabular}{ll}
        (a) $a_1 = 4$, $a_2 = 2$, $a_3 = 0$, $a_4 = -2$ \hspace{0.2in}
            & (b) $b_1 = 3$, $b_2 = 0$, $b_3 = -6$, $b_4 = -18$ \\
        (c) $c_1 = 4$, $c_2 = 10$, $c_3 = 28$, $c_4 = 82$
            & (d) $d_1 = -1$, $d_2 = -4$, $d_3 = -19$, $d_4 = -94$ \\
        (e) $e_0 = 1$, $e_1 = 1$, $e_2 = 6$, $e_3 = 27$
    \end{tabular}
\end{solution}


% Ferland, Sec. 4.1 # 41
\bonusquestion[3] Consider the sequence in problem 1(d).  With $d_1 = -1$ and $d_n = 5\cdot d_{n-1} + 1 \;\;\forall n \geq 2$, the sequence is decreasing; changing the value of the initial condition may change the properties of the sequence.  Determine the smallest value for $d_1$ so that $\{d_n\}$ is not decreasing.
\ifprintanswers
        \vspace{-10pt}
   \fi
\begin{solution}
 An initial condition $d_1 \geq -\frac{1}{4}$ results in a non-decreasing sequence.
\end{solution}



\gquestion{10}{6}{(a,d,e)} Find a closed formula; assume the sequence starts with $n=0, 1, 2, \ldots$.

\begin{tabular}{ll}
    (a) $1, -4, 9, -16, 25, \ldots$ 
        & (b) $3, 6, 12, 24, 48, \ldots$ \\
    (c) $2, 6, 18, 54, 162, 486, 1458\ldots$  \hspace{0.3in}
        & (d) $7, 10, 15, 22, 31, 42, 55, 70, \ldots$ \\
    \multicolumn{2}{c}{(e) $9, 4, -1, -6, -11, \ldots$ }
\end{tabular}
    \ifprintanswers
        \vspace{-10pt}
   \fi
\begin{solution}
    
    \begin{tabular}{lll}
        (a) $a_n = (n+1)^2 (-1)^n$ \hspace{0.6in}
            & (b) $a_n = 3\cdot 2^n$ \hspace{0.6in}
            & (c) $a_n = 2\cdot 3^n$ \\
        (d) $a_n = (n+1)^2 + 6$
            & (e) $a_n = 9 - 5n$
    \end{tabular}
\end{solution}



\gquestion{6}{4}{(a,b)} Find a recursive formula; assume the sequnce starts with $n=0,1,2,\ldots$

\begin{tabular}{ll}
    (a) $3, 6, 12, 24, 48, \ldots$  \hspace{0.3in}
        & (b) $7, 10, 15, 22, 31, 42, 55, 70, \ldots$\\
    \multicolumn{2}{c}{(c) $9, 4, -1, -6, -11, -16, \ldots$}
\end{tabular}
    \ifprintanswers
        \vspace{-10pt}
   \fi
\begin{solution}
    (a) $a_0 = 3$, $a_n = 2*a_{n-1}$ \\
    (b)  $a_0 = 7$, $a_n = a_{n-1} + 2n + 1$  
        \hspace{0.6in} (c) $a_0 = 9$, $a_n = a_{n-1} + -5$
\end{solution}




\gquestion{6}{3}{(a)} Determine whether each answer is a solution to the recurrence relation, 
$$ a_n = a_{n-1} + 2a_{n-2} + 2n - 9 $$
    \begin{enumerate}[label=(\alph*),topsep=0pt,itemsep=0pt,parsep=0pt]
        \item $a_n = 0$
        \item $a_n = -n +2$
    \end{enumerate}
    \ifprintanswers
        \vspace{-10pt}
    \fi
\begin{solution}
    \begin{enumerate}[label=(\alph*),topsep=0pt,itemsep=0pt,parsep=0pt]
        \item Not a solution.
        \begin{align*}
            a_n &= a_{n-1} + 2a_{n-2} + 2n - 9 \\
            &= (0) + 2\cdot0 + 2n - 9 \\
            &= 2n - 9 \\
            0 &\neq 2n - 9
        \end{align*}
        \item Yes, $a_n = -n + 2$ is a solution.
        \begin{align*}
            a_n &= a_{n-1} + 2a_{n-2} + 2n - 9 \\
            &= (-(n-1) + 2) + 2(-(n-2) + 2) + 2n -9 \\
            &= -n + 1 + 2 -2n + 4 + 4 + 2n -9 \\
            &= -n +2 \\
        \end{align*}
    \end{enumerate}
\end{solution}
   

\ugquestion{3} Write out in sigma notation the sum of the first 50 terms of the series: $1 - \frac{1}{2} + \frac{1}{4} - \frac{1}{8} + \frac{1}{16} - \ldots$
    \ifprintanswers
        \vspace{-10pt}
   \fi
\begin{solution}
    The sum can take many form depending on index of summation and limits.  Here are three samples
    
    \begin{center}
    \begin{tabular}{ccc}
        $\ds \sum_{i=1}^{50} (-1)^{n+1}\cdot\frac{1}{2^{n-1}}$ \hspace{0.25in}
        & $\ds \sum_{i=0}^{49} (-1)^{n}\cdot\frac{1}{2^{n}}$ \hspace{0.2in}
        & $\ds \sum_{i=0}^{49} \left(\frac{-1}{2}\right)^n$
    \end{tabular}
    \end{center}
\end{solution}  



\gquestion{15}{10}{(a,e)} Rosen Ch 2.4 \# 16(a,c,e), p. 168.
    \ifprintanswers
        \vspace{-10pt}
   \fi
\begin{solution}
    % \begin{itemize}[itemsep=0pt,parsep=0pt,topsep=0pt,partopsep=0pt]
    %     \item[a)]
        \small \vspace{-0.2in}
        \begin{align*}
            (a) \quad \quad a_n &= -a_{n-1} = -1\cdot a_{n-1} \\
              &= -(-a_{n-2}) = (-1)^2a_{n-2} \\
              &= -(-(-a_{n-3})) = (-1)^3a_{n-3} \\
              &= \cdots \\
              &= (-1)^n\cdot a_{n-n} = (-1)^n\cdot a_{0} = 5\cdot(-1)^n
        \end{align*}
        % \item[(c)] 
        \vspace{-0.1in} 
        \begin{align*}
            (c) \quad \quad a_n &= a_{n-1} - n \\
            &= a_{n-2} -(n-1) - n = a_{n-1} - (n + (n-1)) \\
            &= a_{n-3} -(n-2) - (n + (n-1)) = a_{n-2} - (n + (n-1) + (n-2)) \\
            &= \cdots \\
            &= a_{n-n} -(n + (n-1) + (n-2) + \ldots + (n- (n-1)) \\
            &= a_0 - (n + (n-1) + (n-2) + \ldots + 1) \\
            &= 4 - (n + (n-1) + (n-2) + \ldots + 1) = 4 -\frac{n(n+1)}{2}
        \end{align*}
    % \end{itemize}
        \vspace{-0.1in}
        \begin{align*}
            (e) \quad \quad a_n &= (n+1)a_{n-1} \\
              &= (n+1)na_{n-2} \\
              &= (n+1)n(n-1)a_{n-3} \\
              &= \cdots \\
              &= (n+1)n(n-1)\cdots(n-(n-2))a_{n-n} \\
              &= (n+1)n(n-1)\cdots2a_{0} \\
              &= 2(n+1)!
        \end{align*}
\end{solution}



\gquestion{6}{6}{} A mortage loan is paid off in periodic (monthly) installments, while interest is also charged each period.  A mortage with an annual interest rate of $r$ has a monthly interest rate of $i = \frac{r}{12}$.  A mortage of $M$ dollars at monthly interest rate $i$ has payments of $P$ dollars.  At the end of the month, interest is added to the previous balance, and then the payment $P$ is subtracted from the result.  Let $m_n$ be the balance due after $n$ months, where $m_0 = M$, $m_1 = M(1+i) - P, \ldots$
\begin{enumerate}[label=(\alph*),itemsep=0pt,parsep=0pt,
    topsep=0pt,partopsep=0pt]
    \item Let $M = 10,000$, $i = 0.03$ and $P = 105.13$, determine $m_2$ and $m_3$.
    % \item If $m_{20} = 79,495.98$, $i=0.02$ and $R = 822.89$, determine $m_{21}$.
    \item Find a recursive formula for the mortage balance, $m_n$
\end{enumerate}
    \ifprintanswers
        \vspace{-10pt}
   \fi
\begin{solution}
    \begin{enumerate}[label=(\alph*),itemsep=0pt,parsep=0pt,
    topsep=0pt,partopsep=0pt]
        \item $m_0 = 10,000$, $m_1 = 10194.87$, $m_2 = 10395.59$, $m_3 =  10602.32$
        \item $m_n = m_{n-1}(1+i) - P$, $m_o = M$
    \end{enumerate}
\end{solution}

\ifprintanswers
\else
\newpage
\fi
\uplevel{{\bf Summations}}


\gquestion{18}{9}{(a,c,e)} What are the values of the sums:\\
\begin{tabular}{lll}
    (a) $\ds \sum_{j\in S} (2j - 1), \text{ where } S = \{1, 2, 4, 6\}$
    & (b) $\ds \sum_{i=1}^{8} 4$  \hspace*{1in} 
    & (c) $\ds \sum_{k=0}^{4} (-3)^k$ \\
    & & \\
    (d) $\ds \sum_{j=0}^{7} (2^{j+1} - 2^{j-1})$
    & (e) $\ds \sum_{i=1}^{4} \sum_{j=1}^{3} (2i + 3j)$
    & (f) $\ds \sum_{j=0}^{3} \sum_{k=1}^{3} j*2^{k}$
\end{tabular}
    \ifprintanswers
        \vspace{-10pt}
   \fi
\begin{solution}
    \begin{enumerate}[label=(\alph*),itemsep=0pt,parsep=0pt,
    topsep=0pt,partopsep=0pt]
        \item $(2\cdot1 - 1)+(2\cdot2 - 1)+(2\cdot4 -1)+(2\cdot6-1) = 1+3+7+11 = 22$ 
        \item $\sum_{i=1}^8 4 = 8\cdot4 = 32$
        \item $(-3^0) + (-3^1) + (-3^2) + (-3^3) + (-3^4) = 1 -3 + 9 -27 + 81 = 61 $
        \item $\sum_{j=0}^7 2^{j+1} - \sum_{j=0}^7 2^{j-1} = 510 - 127.5 = 382.5$
        \item $\sum_{i=1}^4 \left( \sum_{j=1}^3 2i + \sum_{j=1}^3 3j \right) = 132$
        \item $\sum_{j=0}^3 \sum_{k=1}^3 j*2^k = 34$
    \end{enumerate}
\end{solution}


\gquestion{8}{8}{} \ifprintanswers 
\else 
A \textit{closed form} of a summation is an equation
in which no summation symbol appears.  The classic example is
$\displaystyle \sum_{i=1}^n i = \frac{n(n+1)}{2}$.  The fraction on
the right is the \textit{closed form} of the summation. 
\fi  For this
problem you will determine closed forms for summation, $\displaystyle \sum_{i=1}^n \sum_{j=1}^n (3i+ 2j)$.  Justify each step using the four facts of the arithmetic properties of summations and Table 2, p. 166 in the book.

\ifprintanswers
\small
\begin{tabular}{llll}
    \multicolumn{2}{l}{Fact} & Example: \\
  Fact 1: & $\displaystyle \sum_{i=1}^n c  = nc$     & Fact 2: & $\displaystyle \sum_{i=j}^n c  = (n-j+1)c$ \\
    & when $c$ is a constant & & when $c$ is a constant \\ 
  Fact 3: & $\displaystyle \sum_{i=j}^n (f(i) \pm g(i)) = \sum_{i=j}^n f(i) \pm \sum_{i=j}^n g(i)$ \hspace{0.2in} & Fact 4: & $\displaystyle \sum_{i=j}^n cf(i) = c \sum_{i=j}^n f(i)$ \\
    & & & when $c$ is a constant \\
\end{tabular}
\else
\small
\begin{tabular}{lll}
    \multicolumn{2}{l}{Fact} & Example: \\
  Fact 1: & $\displaystyle \sum_{i=1}^n c  = nc$     & $\displaystyle \sum_{i=1}^n 7 = 7n$ \\
    & when $c$ is a constant \\
  Fact 2: & $\displaystyle \sum_{i=j}^n c  = (n-j+1)c$  & $\displaystyle \sum_{i=0}^n = 7(n+1) $ \\
    & when $c$ is a constant \\
  Fact 3: & $\displaystyle \sum_{i=j}^n (f(i) \pm g(i)) = \sum_{i=j}^n f(i) \pm \sum_{i=j}^n g(i)$ \hspace{0.2in} &  $\displaystyle \sum_{i=j}^n (2n - n^2) = \sum_{i=j}^n 2n - \sum_{i=j}^n n^2 $ \\
    & \\
  Fact 4: & $\displaystyle \sum_{i=j}^n cf(i) = c \sum_{i=j}^n f(i)$  & $\displaystyle \sum_{i=j}^n (3 \times 2^i) = 3 \sum_{i=j}^n 2^i $ \\
   & when $c$ is a constant \\
\end{tabular}
\fi
    \ifprintanswers
        \vspace{-10pt}
   \fi
\begin{solution}
\begin{tabular}{rll}
  $\displaystyle \sum_{i=1}^n \sum_{j=1}^n (3i+ 2j)$ & $\displaystyle = \sum_{i=1}^n \left[ \sum_{j=1}^n (3i + 2j) \right] $ & add implied parentheses \\
   & $\displaystyle = \sum_{i=1}^n \left[ \sum_{j=1}^n 3i + \sum_{j=1}^n 2j \right]$ & Fact 3 \\
   & $\displaystyle = \sum_{i=1}^n \left[ 3i \sum_{j=1}^n 1 + 2 \sum_{j=1}^n j \right]$ & Fact 4 and Fact 4 \\
   & $\displaystyle = \sum_{i=1}^n \left[ 3i\cdot n + 2 \sum_{j=1}^n j \right]$ & Fact 1  \\
   & $\displaystyle = \sum_{i=1}^n \left[ 3i\cdot n + 2 \cdot \frac{n(n+1)}{2} \right]$ & Table 2 \\
   & $\displaystyle = \sum_{i=1}^n 3i\cdot n + \sum_{i=1}^n n(n+1)$ & Fact 3 \\
   & $\displaystyle = 3n \sum_{i=1}^n i + n(n+1) \sum_{i=1}^n 1$ & Fact 4 (twice) \\
   & $\displaystyle = 3n \cdot \frac{n(n+1)}{2} + n(n+1) \sum_{i=1}^n 1$ & Table 2 \\
   & $\displaystyle = 3n \cdot \frac{n(n+1)}{2} + n(n+1)\cdot n$ & Fact 1 \\
   & $\displaystyle = \frac{5n^2(n+1)}{2} $ & algebra \\
\end{tabular}
\end{solution}

\ugquestion{8} Find a closed form for the summation $\displaystyle \sum_{i=1}^n \sum_{j=1}^n (6i^2 - 2j)$.  Show how you find the closed form solution; justify each step using the four facts of the arithmetic properties of summations and Table 2, p. 166 in the book.
    \ifprintanswers
        \vspace{-10pt}
   \fi
\begin{solution}
\begin{align*}
        \sum_{i=1}^n \sum_{j=1}^n (6i^2 - 2j) 
        &= \sum_{i=1}^n ( \sum_{j=1}^n (6i^2 - 2j) ) \tag{implied parentheses} \\
        &= \sum_{i=1}^n (\sum_{j=1}^n 6i^2 - \sum_{j=1}^n 2j) \tag{Fact 3} \\
        &= \sum_{i=1}^n (6i^2 \sum_{j=1}^n 1 - 2 \sum_{j=1}^n j) \tag{Fact 4, twice} \\
        &= \sum_{i=1}^n (6i^2n - 2 \sum_{j=1}^n j) \tag{Fact 1} \\
        &= \sum_{i=1}^n (6i^2n - 2 \frac{n(n+1)}{2}) \tag{Table 2} \\
        &= \sum_{i=1}^n 6i^2n - \sum_{i=1}^n  n(n+1) \tag{Fact 3} \\
        &= 6n \sum_{i=1}^n i^2 - n(n+1) \sum_{i=1}^n 1 \tag{Fact 4, twice} \\
        &= 6n (\frac{n(n+1)(2n+1)}{6}) - n(n+1) \sum_{i=1}^n 1 \tag{Table 2} \\
        &= n^2(n+1)(2n+1) - n^2(n+1) \tag{algebra} \\
        &= n^2(n+1)(2n + 1  - 1) \\
        &= 2n^3(n+1) 
    \end{align*}
\end{solution}


\ugquestion{4} Rosen Ch 2.4 \#40, p. 169
    \ifprintanswers
        \vspace{-10pt}
   \fi
\begin{solution}
 We can find $\ds \sum_{k=1}^{200} k^3 = \frac{200^2(201)^2}{4}$.
 Also, $\ds \sum_{k=1}^{98} k^3 = \frac{98^2(99)^2}{4}$.

 Therefore,
$$ \sum_{k=99}^{200} = \sum_{k=1}^{200} k^3 - \sum_{k=1}^{98} k^3
   = \frac{200^2(201)^2}{4} - \frac{98^2(99)^2}{4} 
   = 380,477,799 $$
\end{solution}


\uplevel{\textbf{Ch 5 Induction and Recursion}}


\gquestion{8}{8}{} Rosen, Ch 5.1 \# 4, p. 329
    \ifprintanswers
        \vspace{-10pt}
   \fi
\begin{solution}
Let $P(n)$ be the statement that $1^3 + 2^3 + \cdots + n^3 = \left( \frac{n(n+1)}{2} \right)^2$ for the positive integer $n$.
\begin{parts}
    \part (1 point) What is the statement P(1)? \\
        $P(1)$ is the statement $ 1^3 = [ \frac{1 \cdot (1+1) }{2} ]^2 $.
    \part (1 point) Show that P(1) is true, completing the basis step of the proof.
        \[ \left[ \frac{1 \cdot (1+1) }{2} \right]^2 = 1^2 = 1 = 1^3 \]
    \part (2 points) What is the inductive hypothesis? \\
        The inductive hypothesis is to assume $P(k)$ is true for an arbitrary, fixed integer $k \geq 1$, that is
        \[ 1^3 + 2^3 + \cdots + k^3 = \left( \frac{k(k+1)}{2} \right)^2 \]
    \part (2 point) What do you need to prove in the inductive step? \\
        For the inductive step, show for each $k \geq 1$ that $P(k)$ implies $P(k+1)$. \\
        That is, show $P(k+1)$:
        \[ 1^3 + 2^3 + \cdots + k^3 + (k+1)^3 = \left( \frac{(k+1)(k+2)}{2} \right)^2 \]
    \part (3 points) Complete the inductive step. \\
        Since, $P(k)$ holds,
        \begin{align*}
            1^3 + 2^3 + \cdots + k^3 &= \left( \frac{k(k+1)}{2} \right)^2 \tag{Ind. Hyp.} \\
            1^3 + 2^3 + \cdots + k^3 + (k+1)^3 &=  \left( \frac{k(k+1)}{2} \right)^2 + (k+1)^3   \\
              &= \left(\frac{k^2(k+1)^2}{2^2} \right) + (k+1)^3 \\
              &= (k+1)^2 \left( \frac{k^2}{4} + (k + 1) \right) \\
              &= (k+1)^2 \left( \frac{k^2 + 4k + 4}{4} \right) \\
              &= \frac{(k+1)^2(k+2)^2}{2^2} =  \left( \frac{(k+1)(k+2)}{2} \right)^2\\
        \end{align*}
        That is, $1^3 + 2^3 + \cdots +(k+1)^3 = \left( \frac{(k+1)(k+2)}{2} \right)^2 $, the $P(k+1)$ statement.  This completes the inductive step.
    \part (1 point) Explain why these steps show that this formula is true whenever $n$ is a positive integer. \\
        The basis step and inductive step are completed.  Therefore by principle of mathematical induction, the statement is true for every positive integer $n$.
\end{parts}
\end{solution}


% Ferland, p. 189
\ugquestion{8} Use induction to prove the following statement:
    \[\forall n \geq 0, \;\; 4 \,|\, (5^{n} - 1)\]
That is, for the natural numbers, 4 divides $5^n - 1$.
    \ifprintanswers
        \vspace{-10pt}
   \fi
\begin{solution}
Let $P(n)$ be the statement ``4 divides $5^n - 1$" for the natural numbers $n$. 

\textit{Basis Step:} Show $P(0)$ is true. 
    4 does divide $5^n - 1$ where $n=0$;  $4 \,|\, 5^0 - 1 = 1 - 1 = 0$ because there exists an integer $k$ such that $4k = 0$.

\textit{Inductive Step:} \\
\textit{IH} Assume $P(n)$ holds for some $k \geq 0$, that is, there exists an integer $a$ such that $4a = 5^k - 1$. 

Show that $P(k+1)$ holds, that is, there exists an integer $b$ such that $4b = 5^{k+1} - 1$. 

\begin{align*}
    5^{k+1} - 1 &= 5\cdot 5^{k} - 1 \\
     &= (4 + 1)5^{k} - 1 \\
     &= 4\cdot 5^{k} + 5^{k} - 1 \\
     &= 4\cdot 5^{k} + 4a \tag{Ind. Hyp.} \\
     &= 4(5^{k} + a)
     = 4b
\end{align*}
This shows that assuming $P(k)$, $P(k+1)$ holds. \\
Therefore, by completing the basis and inductive step and principle of mathematical induction, the statement $P(n)$ is true for every natural number.
\end{solution}


\end{questions}
\end{document}